f2e: finish lifting of expressions

proof/DDC/Language/SystemF2Effect/VaExpLift.v
@@ -1,4 +1,5 @@
 
+Require Export DDC.Language.SystemF2Effect.TyLift.
 Require Export DDC.Language.SystemF2Effect.VaExpBase.
 Require Export DDC.Base.
 Require Import Coq.Logic.FunctionalExtensionality.
@@ -6,36 +7,133 @@ Require Import Coq.Logic.FunctionalExtensionality.
 
 (********************************************************************)
 (* Lift type indices in expressions. *)
-Fixpoint liftTX (d: nat) (xx: exp) : exp :=
+Fixpoint liftTV (d: nat) (vv: val) : val :=
+  match vv with
+  |  VVar _       => vv
+  |  VLoc _       => vv
+  |  VLam t x     => VLam (liftTT 1 d t) (liftTX d x)
+  |  VLAM k x     => VLAM k              (liftTX (S d) x)
+  |  VConst c     => vv
+  end
+ with liftTX (d: nat) (xx: exp) : exp :=
   match xx with
-  |  XVar _     => xx
-  |  XLoc _     => xx
+  |  XVal v       => XVal   (liftTV d v)
+  |  XLet t x1 x2 => XLet   (liftTT 1 d t)  (liftTX d x1) (liftTX d x2)
+  |  XApp x1 x2   => XApp   (liftTV d x1)   (liftTV d x2)
+  |  XAPP x t     => XAPP   (liftTV d x)    (liftTT 1 d t)
 
-  |  XLAM x     
-  => XLAM (liftTX (S d) x)
+  |  XAlloc t v   => XAlloc (liftTT 1 d t)  (liftTV d v)
+  |  XRead  v     => XRead  (liftTV d v)
+  |  XWrite v1 v2 => XWrite (liftTV d v1)   (liftTV d v2)
 
-  |  XAPP x t 
-  => XAPP (liftTX d x)  (liftTT 1 d t)
- 
-  |  XLam t x   
-  => XLam (liftTT 1 d t)  (liftTX d x)
+  |  XOp1   op1 v => XOp1   op1 (liftTV d v)
+ end.
 
-  |  XApp x1 x2
-  => XApp (liftTX d x1) (liftTX d x2)
 
-  |  XCon dc ts xs
-  => XCon dc (map (liftTT 1 d) ts) (map (liftTX d) xs)
+(********************************************************************)
+(* Lift expression indices in expressions *)
+Fixpoint liftXV (n: nat) (d: nat) (vv: val) {struct vv} : val :=
+  match vv with
+  | VVar ix    
+  => if le_gt_dec d ix
+        (* index was pointing into env, lift it across new elems *)
+        then VVar (ix + n)
+        (* index was locally bound, leave it be *)
+        else vv
 
-  |  XCase xx alts
-  => XCase (liftTX d xx) (map (liftTA d) alts)
+  | VLoc l       => VLoc   l
+  | VLam t1 x1   => VLam   t1 (liftXX n (S d) x1)
+  | VLAM k x     => VLAM   k (liftXX n d x)
+  | VConst c     => VConst c
+  end
+ with   liftXX (n: nat) (d: nat) (xx: exp) {struct xx} : exp :=
+  match xx with 
+  | XVal v       => XVal   (liftXV n d v)
+  | XLet t x1 x2 => XLet t (liftXX n d x1) (liftXX n d x2)
+  | XApp v1 v2   => XApp   (liftXV n d v1) (liftXV n d v2)
+  | XAPP v1 t2   => XAPP   (liftXV n d v1) t2
 
-  |  XUpdate c i ts x1 x2
-  => XUpdate c i (map (liftTT 1 d) ts) (liftTX d x1) (liftTX d x2)
+  | XAlloc t v   => XAlloc t (liftXV n d v)
+  | XRead  v     => XRead  (liftXV n d v)
+  | XWrite v1 v2 => XWrite (liftXV n d v1) (liftXV n d v2)
 
- end
-
- with liftTA (d: nat) (aa: alt) : alt :=
-  match aa with
-  |  AAlt dc xx
-  => AAlt dc (liftTX d xx)
+  | XOp1   op1 v => XOp1   op1 (liftXV n d v)
   end.
+
+
+(********************************************************************)
+(* When we lift an expression by zero places,
+   then the expression is unchanged. *)
+Lemma liftXX_zero
+ : forall d x
+ , liftXX 0 d x = x.
+Proof.
+ intros. gen d.
+ induction x using exp_mutind with 
+  (PV := fun v => forall d
+      ,  liftXV 0 d v = v)
+  ; intros; simpl; try burn.
+
+ Case "XVar".
+  lift_cases; burn.
+Qed.
+Hint Rewrite liftXX_zero : global.
+
+
+(* Commutivity of lifting. *)
+Lemma liftXX_comm
+ : forall n m x d
+ , liftXX n d (liftXX m d x)
+ = liftXX m d (liftXX n d x). 
+Proof.
+ intros. gen d.
+ induction x using exp_mutind with 
+  (PV := fun v => forall d
+      ,  liftXV n d (liftXV m d v)
+      =  liftXV m d (liftXV n d v))
+  ; intros; simpl; try burn.
+
+ Case "XVar".
+  repeat (simple; lift_cases; intros); burn.
+Qed.
+
+
+(* When consecutively lifting an expression, we can lift by one
+   more place in the first lifting and but one less in the second. *)
+Lemma liftXX_succ
+ : forall n m d x
+ , liftXX (S n) d (liftXX m     d x)
+ = liftXX n     d (liftXX (S m) d x). 
+Proof.
+ intros. gen d.
+ induction x using exp_mutind with 
+  (PV := fun v => forall d
+      ,  liftXV (S n) d (liftXV  m    d v)
+      =  liftXV n     d (liftXV (S m) d v))
+  ; intros; simpl; try burn.
+
+ Case "XVar".
+  repeat (simple; lift_cases; intros); burn.
+Qed.
+Hint Rewrite liftXX_succ : global.
+
+
+(* We can collapse two consecutive lifting expressions by lifting 
+   just onces by the sum of the places, provided the lifting
+   occurs at depth zero. *) 
+Lemma liftXX_plus 
+ : forall n m x 
+ , liftXX n 0 (liftXX m 0 x) = liftXX (n + m) 0 x.
+Proof.
+ intros. gen n.
+ induction m; intros.
+  burn.
+
+  intros.
+  rrwrite (n + S m = S n + m). 
+  rewrite liftXX_comm.
+  rewrite <- IHm.
+  rewrite liftXX_comm.
+  burn.
+Qed.
+
